src/cbor/spec/raw/everparse/CBOR.Pulse.Raw.EverParse.Nondet.fsti
@@ -1,0 +1,124 @@
+module CBOR.Pulse.Raw.EverParse.Nondet
+include CBOR.Spec.Raw.Nondet
+open CBOR.Spec.Util
+open CBOR.Spec.Raw.EverParse
+include CBOR.Pulse.Raw.EverParse.Format
+open LowParse.Spec.VCList
+open LowParse.Pulse.VCList
+open Pulse.Lib.Pervasives
+
+module S = Pulse.Lib.Slice.Util
+module SZ = FStar.SizeT
+module Trade = Pulse.Lib.Trade.Util
+
+inline_for_extraction
+let impl_fun_with_invariant_t
+  (#t: Type)
+  (f: (x1: raw_data_item) -> t)
+  (inv: slprop)
+=
+  (l1: S.slice byte) ->
+  (#p1: perm) ->
+  (#gl1: Ghost.erased (raw_data_item)) ->
+  stt t
+    (inv ** pts_to_serialized (serialize_raw_data_item) l1 #p1 gl1)
+    (fun res ->
+      inv ** pts_to_serialized (serialize_raw_data_item) l1 #p1 gl1 **
+      pure (
+        res == f gl1
+      )
+    )
+
+inline_for_extraction
+let impl_equiv_t
+  (#t: Type)
+  (equiv: (x1: raw_data_item) -> (x2: raw_data_item) -> t)
+=
+  (l1: S.slice byte) ->
+  (#p1: perm) ->
+  (#gl1: Ghost.erased (raw_data_item)) ->
+  impl_fun_with_invariant_t
+    (equiv gl1)
+    (pts_to_serialized (serialize_raw_data_item) l1 #p1 gl1)
+
+let option_sz_v (x: option SZ.t) : GTot (option nat) =
+  match x with
+  | None -> None
+  | Some x' -> Some (SZ.v x')
+
+inline_for_extraction
+let impl_equiv_hd_t
+  (#t: Type)
+  (equiv: (x1: raw_data_item) -> (x2: raw_data_item) -> t)
+=
+  (n1: Ghost.erased nat) ->
+  (l1: S.slice byte) ->
+  (n2: Ghost.erased nat) ->
+  (l2: S.slice byte) ->
+  (#p1: perm) ->
+  (#gl1: Ghost.erased (nlist n1 raw_data_item)) ->
+  (#p2: perm) ->
+  (#gl2: Ghost.erased (nlist n2 raw_data_item)) ->
+  stt t
+    (pts_to_serialized (serialize_nlist n1 serialize_raw_data_item) l1 #p1 gl1 **
+      pts_to_serialized (serialize_nlist n2 serialize_raw_data_item) l2 #p2 gl2 **
+      pure (
+        n1 > 0 /\ n2 > 0
+      )
+    )
+    (fun res ->
+pts_to_serialized (serialize_nlist n1 serialize_raw_data_item) l1 #p1 gl1 **
+      pts_to_serialized (serialize_nlist n2 serialize_raw_data_item) l2 #p2 gl2 **
+      pure (
+        n1 > 0 /\ n2 > 0 /\
+        res == equiv (List.Tot.hd gl1) (List.Tot.hd gl2)
+      )
+    )
+
+inline_for_extraction
+let impl_check_equiv_map_hd_t
+  (data_model: (raw_data_item -> raw_data_item -> bool))
+=
+  (map_bound: option SZ.t) ->
+  impl_equiv_hd_t (check_equiv_map data_model (option_sz_v map_bound))
+
+inline_for_extraction
+val impl_check_equiv_map_hd_body
+  (#data_model: Ghost.erased ((x1: raw_data_item) -> (x2: raw_data_item) -> bool))
+  (impl_data_model: impl_equiv_hd_t data_model)
+  (impl_check_equiv_map_hd: impl_check_equiv_map_hd_t data_model)
+: impl_check_equiv_map_hd_t (Ghost.reveal data_model)
+
+inline_for_extraction
+val impl_check_equiv
+  (#data_model: Ghost.erased ((x1: raw_data_item) -> (x2: raw_data_item) -> bool))
+  (impl_check_equiv_map_hd: impl_check_equiv_map_hd_t data_model)
+  (map_bound: option SZ.t)
+: impl_equiv_t #_ (check_equiv data_model (option_sz_v map_bound))
+
+val impl_check_map_depth
+  (bound: SZ.t)
+  (n0: SZ.t)
+  (l0: S.slice byte)
+  (#pm: perm)
+  (#gl0: Ghost.erased (nlist (SZ.v n0) raw_data_item))
+: stt bool
+(requires
+  pts_to_serialized (serialize_nlist (SZ.v n0) serialize_raw_data_item) l0 #pm gl0
+)
+(ensures fun res ->
+  pts_to_serialized (serialize_nlist (SZ.v n0) serialize_raw_data_item) l0 #pm gl0 **
+  pure (
+    res == check_map_depth (SZ.v bound) gl0
+  )
+)
+
+inline_for_extraction
+val impl_check_valid
+  (#data_model: Ghost.erased ((x1: raw_data_item) -> (x2: raw_data_item) -> bool))
+  (map_bound: option SZ.t)
+  (impl_check_equiv: impl_equiv_t #_ (check_equiv data_model (option_sz_v map_bound)))
+  (strict_bound_check: bool)
+: impl_fun_with_invariant_t #_
+    (check_valid data_model (option_sz_v map_bound) strict_bound_check)
+    emp
